Add 'iLDestruct' tactic to more efficiently destruct list of (possibly) named assertions. Use with logging example.

src/CSL/NamedDestruct.v
@@ -17,7 +17,14 @@ Export ident.
 Definition named_def {PROP: bi} (i: ident) (H: PROP) : PROP := H.
 Definition named_aux {PROP: bi} : seal (@named_def PROP). by eexists. Qed.
 Definition named {PROP: bi} := (@named_aux PROP).(unseal).
-Definition named_eq {PROP : bi} := (@named_aux PROP).(seal_eq).
+Definition named_eq {PROP : bi} : @named PROP = @named_def PROP := (@named_aux PROP).(seal_eq).
+
+Global Instance named_timeless {PROP: sbi} i (P: PROP) : Timeless P → Timeless (named i P).
+Proof. rewrite named_eq /named_def//=. Qed.
+
+Global Instance named_frame_here :
+  ∀ (PROP : bi) i (p : bool) (R : PROP), Frame p (named i R) R emp | 100.
+Proof. intros ???. rewrite named_eq /named_def //=//=. apply _. Qed.
 
 Fixpoint env_bundle_names {PROP: bi} (Γ: env PROP) : env PROP :=
   match Γ with
@@ -34,7 +41,7 @@ Lemma envs_bundle_names_sound {PROP: bi} (Δ: envs PROP) :
 Proof.
   destruct Δ as (Γp,Γs,p). rewrite /envs_bundle_names.
   f_equal.
-  induction Γs; rewrite //= /named named_eq /named_def IHΓs //=.
+  induction Γs; rewrite //= named_eq /named_def IHΓs //=.
 Qed.
 
 Lemma tac_bundle_names {PROP: bi} (Δ: envs PROP) Q :
@@ -51,7 +58,7 @@ Ltac bundle_names :=
 
 (* TODO: this is not very robust. *)
 Ltac unbundle_names :=
-  rewrite /named ?named_eq;
+  rewrite ?named_eq;
   match goal with |- ?u => let v := eval cbv [named_def] in u in change v end.
 
 Ltac iAssignNames :=
@@ -86,11 +93,146 @@ Ltac iDestructRepR H :=
 Ltac iDestructIntro :=
   let H := iFresh in iIntros H; iDestructExRep H; iAssignNames.
 
+Inductive LTag : Set :=
+| LNamed : string → LTag
+| LAnon : LTag.
+Coercion LNamed : string >-> LTag.
+
+Definition tagged_prop (PROP: bi) := (LTag * PROP)%type.
+Definition tagged_to_prop {PROP} (tP: tagged_prop PROP) : PROP :=
+  match tP with
+  | (LNamed s, P) => named s P
+  | (LAnon, P) => P
+  end.
+Definition prop_list (PROP: bi) := list (tagged_prop PROP).
+Definition pl2p {PROP : bi} (Ps: prop_list PROP) : list PROP := map (tagged_to_prop) Ps.
+Definition pl2pp {PROP : bi} (Ps: prop_list PROP) := ([∗] (pl2p Ps))%I.
+
+
+Class IntoSepEnv {PROP : bi} (P: PROP) (Ps: prop_list PROP) :=
+  into_sep_env : P ⊢ [∗] (pl2p Ps).
+Arguments IntoSepEnv {_} _%I _%I : simpl never.
+Arguments into_sep_env {_} _%I _%I {_}.
+Hint Mode IntoSepEnv + ! - : typeclass_instances.
+
+Definition envs_set_counter {PROP} (Δ : envs PROP) (p: positive) : envs PROP :=
+  Envs (env_intuitionistic Δ) (env_spatial Δ) p.
+Lemma envs_set_counter_equiv {PROP} (Δ : envs PROP) p : envs_Forall2 (⊣⊢) Δ (envs_set_counter Δ p).
+Proof. done. Qed.
+Lemma envs_set_counter_sound {PROP} (Δ: envs PROP) p : of_envs (envs_set_counter Δ p) ⊣⊢ of_envs Δ.
+Proof. by f_equiv. Qed.
+
+Section list_destruct.
+Context {PROP: bi}.
+Fixpoint pl_env_expand (p: positive) (Ps: prop_list PROP) (Γ: env PROP) : positive * env PROP :=
+  match Ps with
+  | nil => (p, Γ)
+  | (LAnon, P) :: Ps' => pl_env_expand (Pos_succ p) Ps' (Esnoc Γ (IAnon p) P)
+  | (LNamed s, P) :: Ps' => pl_env_expand p Ps' (Esnoc Γ s P)
+  end.
+Global Instance env_into_sep_env (Ps: prop_list PROP) : IntoSepEnv ([∗] pl2p Ps) Ps.
+Proof. rewrite /IntoSepEnv. trivial. Qed.
+
+Global Instance sep_into_sep_single_named (i: string) (P: PROP) :
+  IntoSepEnv (named i P) [(LNamed i, P)].
+Proof. rewrite /IntoSepEnv//=. iFrame. eauto. Qed.
+
+Global Instance sep_into_sep_cons (i: string) (P Q: PROP) Ps :
+  IntoSepEnv Q Ps →
+  IntoSepEnv (named i P ∗ Q) ((LNamed i, P) :: Ps).
+Proof. rewrite /IntoSepEnv//=. iIntros (H1) "(?&?)". iFrame. by iApply H1. Qed.
+
+Global Instance sep_into_sep_single_anon (P: PROP) :
+  IntoSepEnv P [(LAnon, P)] | 100.
+Proof. rewrite /IntoSepEnv//=. iFrame. eauto. Qed.
+
+Lemma tac_sep_list_destruct Δ Δ' i Γ bump (P: PROP) (Ps: prop_list PROP) Q :
+  envs_lookup i Δ = Some (false, P) →
+  IntoSepEnv P Ps →
+  pl_env_expand (env_counter Δ) Ps Enil = (bump, Γ) →
+  envs_simple_replace i false Γ Δ = Some Δ' →
+  envs_entails (envs_set_counter Δ' bump) Q → envs_entails Δ Q.
+Proof.
+  rewrite envs_entails_eq => Hlookup Hsep Hexpand Hrepl Himpl.
+  rewrite envs_simple_replace_sound //=.
+  rewrite /= (into_sep_env P).
+  assert (Hrec: ∀ p (Γ: env PROP), ([∗] Γ -∗ [∗] pl2p Ps -∗ [∗] snd (pl_env_expand p Ps Γ))%I).
+  { clear. induction Ps => //= p Γ.
+    * iIntros "H"; eauto.
+    * iIntros "H1 (a&H2)".
+      destruct a as ([]&?); simpl;
+      iApply (IHPs with "[a H1] H2"); iFrame.
+  }
+  specialize (Hrec (env_counter Δ) Enil). rewrite Hexpand in Hrec.
+  iIntros "(HPs&HIH)". iPoseProof (Hrec with "[$] [$]") as "HPs'".
+  rewrite envs_set_counter_sound in Himpl * => ->.
+  by iApply "HIH".
+Qed.
+End list_destruct.
+
+Ltac set_counter_reduce :=
+  match goal with |- ?u => let v := eval cbv [envs_set_counter] in u in change v end.
+
+Ltac iLDestruct H :=
+  eapply (tac_sep_list_destruct _ _ H);
+  [pm_reflexivity ||
+     let H := pretty_ident H in
+     fail "iLDestruct:" H "not found"
+  |apply _
+  |pm_reflexivity ||
+     fail "iLDestruct: some name not fresh"
+  |pm_reflexivity ||
+     fail "iLDestruct: some name not fresh"
+  |set_counter_reduce; pm_reduce].
+
+Ltac iLIntro :=
+  let H := iFresh in iIntros H; iLDestruct H.
+
 Section test.
-Context {PROP : bi}.
+Context {PROP: bi}.
 Context {P P' : PROP}.
 
 Context (HPP': P ⊢ P').
+
+Definition test_list := pl2p [ (LNamed "Hfoo", P); (LAnon, P')  ].
+Fixpoint bigterm_list (P: PROP) n :=
+  match n with
+  | O => []
+  | S n' => (LAnon, P) :: bigterm_list P n'
+  end.
+
+Lemma HPP_destruct_named : True ∗ [∗] test_list ∗ True ⊢ P -∗ P -∗ P -∗ P -∗ [∗] test_list.
+Proof.
+  iIntros "(?&H0&H1)".
+  iLDestruct "H0".
+Abort.
+
+Lemma HPP_intro_named : [∗] test_list ⊢ P -∗ P -∗ P -∗ P -∗ [∗] test_list.
+Proof.
+  iLIntro.
+Abort.
+
+Lemma Hbig : [∗] (pl2p (bigterm_list P 20)) ⊢ True.
+Proof.
+  iLIntro.
+  auto.
+Qed.
+
+(*
+Lemma Hbig_slow : [∗] (pl2p (bigterm_list P 20)) ⊢ True.
+Proof.
+  simpl.
+  iDestructIntro.
+  auto.
+Qed.
+*)
+
+Lemma Hbig_combined : [∗] (pl2p (bigterm_list P 20)) -∗ [∗] (pl2p (bigterm_list P 20)) -∗ True.
+  iLIntro.
+  iLIntro.
+  auto.
+Qed.
+
 Lemma HPP_named i : named i P ⊢ named i P'.
 Proof using HPP'. by unbundle_names. Qed.
 
@@ -106,5 +248,4 @@ Lemma test2 Q: (named "HP" P) ∗ (named "HQ" Q) ⊢ P ∗ Q.
 Proof using HPP'.
   iDestructIntro. iFrame "HP". iFrame "HQ".
 Qed.
-
 End test.
